regex/Regex/Data/Anchor.lean
@@ -1,0 +1,13 @@
+namespace Regex.Data
+
+inductive Anchor where
+  | start
+  | eos
+deriving DecidableEq, Repr, Inhabited
+
+def Anchor.test (it : String.Iterator) (anchor : Anchor) : Bool :=
+  match anchor with
+  | Anchor.start => it.pos = 0
+  | Anchor.eos => it.atEnd
+
+end Regex.Data
